Induction principle for partitionImpl

QuickSortInLean/QuickSort.lean
@@ -7,7 +7,7 @@ theorem Nat.le_sub_of_lt {m n : Nat} (h : m < n) : m ≤ n - 1 := by
     apply Nat.le_trans ih
     apply Nat.sub_le_succ_sub
 
-def partitionImpl {α : Type} [Ord α]
+def partitionImpl {α : Type} [inst : LT α] [DecidableRel inst.lt]
   {n : Nat} (arr : Vec α n) (first i j : Nat)
   (fi : first ≤ i) (ij : i ≤ j) (jn : j < n) :
   { mid : Nat // first ≤ mid ∧ mid ≤ j } × Vec α n :=
@@ -15,11 +15,10 @@ def partitionImpl {α : Type} [Ord α]
   have : first < n := Nat.lt_of_le_of_lt fi this
   if fi : first < i then
     have : first ≤ i - 1 := Nat.le_sub_of_lt fi
-    match compare arr[i] arr[first] with
-    | .lt =>
+    if arr[i] < arr[first] then
       have : i - 1 ≤ j := Nat.le_trans (Nat.sub_le ..) ij
       partitionImpl arr first (i - 1) j (by assumption) (by assumption) jn
-    | .eq | .gt =>
+    else
       have : i - 1 ≤ j - 1 := Nat.sub_le_sub_right ij 1
       have : j - 1 < n := Nat.lt_of_le_of_lt (Nat.sub_le ..) jn
       let arr := (dbgTraceIfShared "swap1" arr).swap ⟨i, by assumption⟩ ⟨j, jn⟩
@@ -27,9 +26,9 @@ def partitionImpl {α : Type} [Ord α]
       | (⟨mid, hm⟩, arr) => (⟨mid, ⟨hm.1, Nat.le_trans hm.2 (Nat.sub_le ..)⟩⟩, arr)
   else
     let arr := (dbgTraceIfShared "swap2" arr).swap ⟨first, by assumption⟩ ⟨j, by assumption⟩
-    (⟨j, And.intro (Nat.le_trans (by assumption) ij) (by simp)⟩, arr)
+    (⟨j, ⟨Nat.le_trans (by assumption) ij, by simp⟩⟩, arr)
 
-def partition {α : Type} [Ord α]
+def partition {α : Type} [inst : LT α] [DecidableRel inst.lt]
   {n : Nat} (arr : Vec α n) (first last : Nat)
   (fl : first ≤ last) (ln : last < n) :
   { mid : Nat // first ≤ mid ∧ mid ≤ last } × Vec α n :=
@@ -48,7 +47,7 @@ theorem Nat.lt_sub_right {m n k : Nat} (mk : k ≤ m) (mn : m < n) : m - k < n -
   rw [this]
   apply Nat.sub_le_sub_right mn
 
-def quickSortImpl {α : Type} [Ord α]
+def quickSortImpl {α : Type} [inst : LT α] [DecidableRel inst.lt]
   {n : Nat} (arr : Vec α n) (first last : Nat) (ln : last < n) :
   Vec α n :=
   if lt : first < last then
@@ -81,13 +80,13 @@ where
       exact Nat.lt_sub_right (by assumption) (Nat.lt_of_lt_of_le (by assumption) hmid₂)
 termination_by _ => last - first
 
-def quickSort' {α : Type} [Ord α] {n : Nat} (arr : Vec α n) : Vec α n :=
+def quickSort' {α : Type} [inst : LT α] [DecidableRel inst.lt] {n : Nat} (arr : Vec α n) : Vec α n :=
   if _ : n > 0 then
     quickSortImpl arr 0 (n - 1) (Nat.sub_lt (by assumption) (by decide))
   else
     arr
 
-def quickSort {α : Type} [Ord α] (arr : Array α) : Array α :=
+def quickSort {α : Type} [inst : LT α] [DecidableRel inst.lt] (arr : Array α) : Array α :=
   (quickSort' (n := arr.size) arr).val
 
 -- #eval quickSort #[7, 5, 6, 2, 8, 1, 9, 4, 10, 3]
